---
title: "P8108 Homework 5"
author: "Ryan Wei, rw2844"
date: "2022-10-12"
output: pdf_document
---

```{r setup, include=FALSE}
knitr::opts_chunk$set(echo = FALSE, message = FALSE, warning = FALSE)
```

## Problem 3

**Proof**

Since $T_i\sim Exp(h_i), T_j \sim Exp(h_j)$, we can get
$$
\begin{aligned}
f_{T_i}(t) & = h_i\exp(-h_it)\\
f_{T_j}(t) & = h_i\exp(-h_jt)
\end{aligned}
$$

Hence
$$
\begin{aligned}
P(T_i\ge T_j) & = 1 - P(T_i < T_j) \\
& = 1 - \left(\int_{0}^{\infty}P(T_i < T_j\mid T_j = v)f_{T_j}(v)dv\right)\\
& = 1 - \left(\int_{0}^{\infty}\int_0^{v}f_{T_i}(u)f_{T_j}(v)dudv\right) & \text{(since }T_i\perp T_j\text{)}\\
& = 1 - \left(\int_{0}^{\infty}(1-\exp(-h_iv))h_j\exp(-h_jv)dv\right)\\
& = 1- \left(\int_{0}^{\infty}h_j\exp(-h_jv)dv- \frac{h_j}{h_i+h_j}\int_{0}^{\infty}(h_i+h_j)\exp(-(h_i+h_j)v)dv\right)\\
& = 1 - \left(1 - \frac{h_j}{h_i+h_j} \right)\\
& = \frac{h_j}{h_i+h_j}
\end{aligned}
$$
\hfill$\square$